src/SymI.v
@@ -1,0 +1,87 @@
+Require Import MirrorCore.ExprI.
+Require Import MirrorCore.TypesI.
+
+Set Implicit Arguments.
+Set Strict Implicit.
+
+Section symbols.
+  Variable typ : Type.
+  Variable typD : list Type -> typ -> Type.
+  Variable func : Type.
+
+  Class RSym : Type :=
+  { typeof_sym : func -> option typ
+  ; symD : forall f : func, match typeof_sym f with
+                               | None => unit
+                               | Some t => typD nil t
+                             end
+  }.
+
+  Context {RType_typ : RType typD}.
+  Context {RSym_func : RSym}.
+
+  Definition funcAs (f : func) (t : typ) : option (typD nil t) :=
+    match typeof_sym f as ft
+          return match ft with
+                   | None => unit
+                   | Some t => typD nil t
+                 end -> option (typD nil t)
+    with
+      | None => fun _ => None
+      | Some ft => fun val =>
+        match typ_cast (fun x => x) nil ft t with
+          | None => None
+          | Some cast => Some (cast val)
+        end
+    end (symD f).
+
+  Context {RTypeOk_typ : RTypeOk RType_typ}.
+
+  Theorem funcAs_Some : forall f t (pf : typeof_sym f = Some t),
+    funcAs f t =
+    Some match pf in _ = z return match z with
+                                    | None => unit
+                                    | Some z => typD nil z
+                                  end with
+           | eq_refl => symD f
+         end.
+  Proof.
+    intros. unfold funcAs.
+    generalize (symD f).
+    rewrite pf. intros.
+    destruct (typ_cast_refl nil t (fun x => x)).
+    intuition.
+    match goal with
+      | H : ?Y = _ |- match ?X with _ => _ end = _ =>
+        change X with Y ; rewrite H
+    end; intros.
+    f_equal. eauto.
+  Qed.
+
+  (** This helper function makes it a little bit easier to construct
+   ** [RSym] instances by not requiring the split. It is a little bit less
+   ** efficient in some instances in some cases where type checking can
+   ** be done independently of determining the denotation function.
+   **)
+  Definition RSym_from (fd : func -> option {t : typ & typD nil t}) : RSym :=
+  {| typeof_sym := fun f =>
+                    match fd f with
+                      | None => None
+                      | Some (existT t _) => Some t
+                    end
+   ; symD := fun f =>
+               match fd f as F return match match F with
+                                              | None => None
+                                              | Some (existT t _) => Some t
+                                            end
+                                      with
+                                        | None => unit
+                                        | Some t => typD nil t
+                                      end
+               with
+                 | None => tt
+                 | Some (existT t d) => d
+               end
+   |}.
+
+End symbols.
